m

DynamoDbItemEncryptor/src/DynamoToStruct.dfy
@@ -110,22 +110,37 @@ module DynamoToStruct {
 
   type AttrNameAndSerializedValue = (AttributeName, seq<uint8>)
 
-  predicate method AttrLexicographicLessOrEqual(x : AttrNameAndSerializedValue, y : AttrNameAndSerializedValue)
-  {
+  predicate method CharLess(x : char, y : char) {
+    x < y
+  }
+  predicate method ByteLess(x : uint8, y : uint8) {
+    x < y
+  }
+
+  predicate method AttrLexicographicLessOrEqual(x : AttrNameAndSerializedValue, y : AttrNameAndSerializedValue) {
     LexicographicLessOrEqual(x.0, y.0, CharLess)
   }
 
-  predicate method StringLexicographicLessOrEqual(x : string, y : string)
-  {
+  predicate method StringLexicographicLessOrEqual(x : string, y : string) {
     LexicographicLessOrEqual(x, y, CharLess)
+  }
+
+  predicate method ByteLexicographicLessOrEqual(x : seq<uint8>, y : seq<uint8>) {
+    LexicographicLessOrEqual(x, y, ByteLess)
   }
 
 /*
   We know this is a total order, because LexicographicLessOrEqual on strings is a total order
   TODO - actually prove it
+
+  I am assured that a solution to this will be pushed to the Dafny standard library by December 9th.
 */
   lemma {:axiom} AttrLexicographicLessOrEqualIsTotal()
     ensures TotalOrdering(AttrLexicographicLessOrEqual)
+  lemma {:axiom} StringLexicographicLessOrEqualIsTotal()
+    ensures TotalOrdering(StringLexicographicLessOrEqual)
+  lemma {:axiom} ByteLexicographicLessOrEqualIsTotal()
+    ensures TotalOrdering(ByteLexicographicLessOrEqual)
 /*
   {
     assert Reflexive(AttrLexicographicLessOrEqualIsTotal);
@@ -163,15 +178,20 @@ module DynamoToStruct {
       case N(n) => Wrap(a, wrap, UTF8.Encode(n))
       case B(b) => Wrap(a, wrap, Success(b))
       case SS(ss) =>
-        //var ss := MergeSortBy(ss, StringLexicographicLessOrEqual);
+        StringLexicographicLessOrEqualIsTotal();
+        var ss := MergeSortBy(ss, StringLexicographicLessOrEqual);
         var count :- U32ToBigEndian(|ss|);
         var body :- CollectString(ss);
         Wrap(a, wrap, Success(count + body))
       case NS(ns) =>
+        StringLexicographicLessOrEqualIsTotal();
+        var ns := MergeSortBy(ns, StringLexicographicLessOrEqual);
         var count :- U32ToBigEndian(|ns|);
         var body :- CollectString(ns);
         Wrap(a, wrap, Success(count + body))
       case BS(bs) =>
+        ByteLexicographicLessOrEqualIsTotal();
+        var bs := MergeSortBy(bs, ByteLexicographicLessOrEqual);
         var count :- U32ToBigEndian(|bs|);
         var body :- CollectBinary(bs);
         Wrap(a, wrap, Success(count + body))
@@ -218,9 +238,13 @@ module DynamoToStruct {
       Success(SeqToUInt32(x[..4]) as nat)
   }
   
+  predicate IsSorted<T>(s: seq<T>, lessThanOrEq: (T, T) -> bool) {
+    forall j, k :: 0 <= j < k < |s| ==> lessThanOrEq(s[j], s[k])
+  }
+
   // String Set or Number Set to Bytes
   function method {:tailrecursion} CollectString(b : StringSetAttributeValue, acc : seq<uint8> := []) : Result<seq<uint8>, string>
-    // requires sorted, ensures sorted
+    requires IsSorted(b, StringLexicographicLessOrEqual)
   {
     if |b| == 0 then
       Success(acc)
@@ -232,7 +256,7 @@ module DynamoToStruct {
 
   // Binary Set to Bytes
   function method {:tailrecursion} CollectBinary(b : BinarySetAttributeValue, acc : seq<uint8> := []) : Result<seq<uint8>, string>
-  // requires sorted, ensures sorted
+    requires IsSorted(b, ByteLexicographicLessOrEqual)
   {
     if |b| == 0 then
       Success(acc)
@@ -256,7 +280,7 @@ module DynamoToStruct {
   // Map to Bytes
   // input sequence is already serialized
   function method {:tailrecursion} CollectMap(b : seq<AttrNameAndSerializedValue>, acc : seq<uint8> := []) : Result<seq<uint8>, string>
-      // requires sorted, ensures sorted
+    requires IsSorted(b, AttrLexicographicLessOrEqual)
   {
     if |b| == 0 then
       Success(acc)
@@ -519,11 +543,6 @@ module DynamoToStruct {
     else
       Failure("Unsupported TerminalTypeId")
   
-  }
-  
-  predicate method CharLess(x : char, y : char)
-  {
-    x < y
   }
 
   // Turn a map<Result<X,string>, Result<Y,string>> into a Result<map<X,Y>, string>
